# Sorting

```
module Permutations where

open import Data.Nat using (â„•)
import Data.Nat as â„•
import Data.Nat.Properties as â„•
open import Data.Fin renaming (Fin to ğ”½)
open import Data.Fin.Properties hiding (setoid)
open import Function.Inverse
open import Relation.Binary.PropositionalEquality using (_â‰¡_; refl; cong; module â‰¡-Reasoning)
open import Relation.Nullary
open import Function.LeftInverse
open import Function.Equality using (_âŸ¶_)
open import Level using (0â„“)
open import Relation.Binary.Bundles
open import Data.Product

Perm : â„• â†’ Set
Perm n = ğ”½ n â†” ğ”½ n

-- ğ”½(m + n) â‡” ğ”½(m) âŠ ğ”½(n) â‡” ğ”½(n) âŠ ğ”½(m) â‡” ğ”½(n + m)
--


-- vocabulary
-- mathematical properties give you ways to prove things



-- (02) --
-- (13) --

+1-mod-n : {n : â„•} â†’ ğ”½ n â†’ ğ”½ n
+1-mod-n {â„•.suc n} m with n â„•.â‰Ÿ toâ„• m
... | no mâ‰¢n  = suc (lowerâ‚ m mâ‰¢n)
... | yes _ = zero

-1-mod-n : {n : â„•} â†’ ğ”½ n â†’ ğ”½ n
-1-mod-n {â„•.suc n} zero = fromâ„• n
-1-mod-n {â„•.suc n} (suc m) = injectâ‚ m


iâ‰¡jâ‡’j<i+1 : âˆ€ {i j } â†’ i â‰¡ j â†’ j â„•.< â„•.suc i
iâ‰¡jâ‡’j<i+1 {i} {j} iâ‰¡j =
  begin
    â„•.suc j
  â‰¡âŸ¨ cong â„•.suc (â‰¡-sym iâ‰¡j) âŸ©
    â„•.suc i
  âˆ
  where
    open Relation.Binary.PropositionalEquality renaming (sym to â‰¡-sym)
    open â„•.â‰¤-Reasoning

open â‰¡-Reasoning

left-inverseâ€² : (n : â„•) â†’ (x : ğ”½ n) â†’ -1-mod-n (+1-mod-n x) â‰¡ x
left-inverseâ€² â„•.zero ()
left-inverseâ€² (â„•.suc â„•.zero) zero = refl
left-inverseâ€² (â„•.suc (â„•.suc nâ€²)) x
            with â„•.suc nâ€² â„•.â‰Ÿ toâ„• x
...  | no n+1â‰¢x with x
...               | zero = refl
...               | suc x =
    begin
      -1-mod-n (suc (lowerâ‚ (suc x) n+1â‰¢x))
    â‰¡âŸ¨âŸ©
      injectâ‚ (lowerâ‚ (suc x) n+1â‰¢x)
    â‰¡âŸ¨  injectâ‚-lowerâ‚ (suc x) n+1â‰¢x âŸ©
      suc x
    âˆ
left-inverseâ€² (â„•.suc (â„•.suc n)) x
     | yes n+1â‰¡x =
   begin
     -1-mod-n zero
   â‰¡âŸ¨âŸ©
     fromâ„• (â„•.suc n)
   â‰¡âŸ¨ fromâ„•-def (â„•.suc n) âŸ©
     fromâ„•< n+1<n+2
   â‰¡âŸ¨ fromâ„•<-cong (â„•.suc n) (toâ„• x) n+1â‰¡x n+1<n+2 (iâ‰¡jâ‡’j<i+1 n+1â‰¡x) âŸ©
      fromâ„•< (iâ‰¡jâ‡’j<i+1 n+1â‰¡x )
   â‰¡âŸ¨ fromâ„•<-toâ„• x (iâ‰¡jâ‡’j<i+1 n+1â‰¡x)  âŸ©
     x
   âˆ
   where
     n+1<n+2 : â„•.suc n â„•.< â„•.suc (â„•.suc n)
     n+1<n+2 = â„•.sâ‰¤s (â„•.sâ‰¤s (â„•.â‰¤-reflexive refl))

{- right-inverseâ€² : (n : â„•) â†’ (x : ğ”½ n) â†’ +1-mod-nâ€² (-1-mod-n x) â‰¡ x
right-inverseâ€² (â„•.suc n) zero
  with fromâ„• n â‰Ÿ fromâ„• n
... | yes _ =
  begin
    +1-mod-nâ€² (-1-mod-n zero)
  â‰¡âŸ¨ {!!} âŸ©
    zero
  âˆ
-}


module PermGroup (n : â„•) where
  open import Algebra.Structures {A = Perm n } _â‰¡_
  open import Algebra.Definitions {A = Perm n } _â‰¡_
  open import Relation.Binary.PropositionalEquality

  identity : Perm n
  identity =
      record
        { to = record { _âŸ¨$âŸ©_ = Î» x â†’ x ; cong = Î» z â†’ z }
        ; from = record { _âŸ¨$âŸ©_ = Î» x â†’ x ; cong = Î» z â†’ z }
        ; inverse-of =
            record
               { left-inverse-of = left-inverse
               ; right-inverse-of = right-inverse
               }
        }
    where
      open â‰¡-Reasoning
      left-inverse : (x : ğ”½ n) â†’ x â‰¡ x
      left-inverse _ = refl

      right-inverse : (x : ğ”½ n) â†’ x â‰¡ x
      right-inverse _ = refl

  sucPred : Perm n
  sucPred =
    record
      { to = toâ€²
      ; from = fromâ€²
      ; inverse-of =
          record
            { left-inverse-of = left-inverse
            ; right-inverse-of = right-inverse
            }
      }
    where
       open â‰¡-Reasoning
       to-cong : âˆ€ {i j} â†’ i â‰¡ j â†’ +1-mod-n i â‰¡ +1-mod-n j
       to-cong refl = refl

       from-cong : âˆ€ {i j} â†’ i â‰¡ j â†’ -1-mod-n i â‰¡ -1-mod-n j
       from-cong refl = refl

       toâ€² : setoid (ğ”½ n) âŸ¶ setoid (ğ”½ n)
       toâ€² = record
               { _âŸ¨$âŸ©_ = +1-mod-n
               ; cong = to-cong
               }

       fromâ€² : setoid (ğ”½ n) âŸ¶ setoid (ğ”½ n)
       fromâ€² = record
            { _âŸ¨$âŸ©_ = -1-mod-n
            ; cong = from-cong
            }


       left-inverse : (x : ğ”½ n) â†’ -1-mod-n (+1-mod-n x) â‰¡ x
       left-inverse x = left-inverseâ€² n x

       right-inverse : (x : ğ”½ n) â†’ +1-mod-n (-1-mod-n x) â‰¡ x
       right-inverse = {!!}
```
